daily save

compiler/backend/passes/proofs/thunk_combine_Forcing_LambdasScript.sml
@@ -49,19 +49,52 @@ Inductive exp_rel:
      exp_rel x1 x2 ∧
      exp_rel y1 y2 ⇒
      exp_rel (Let opt x1 y1) (Let opt x2 y2)) ∧
-[~Let_Lams_combine:]
-  (∀v1 v2 vL bL1 bL2 x1 x2 y1 y2 i.
-     LENGTH vL = LENGTH bL2 ∧
-     ¬MEM v1 vL ∧ ALL_DISTINCT vL ∧ vL ≠ [] ∧
-     i < LENGTH vL ∧ (∀j. j ≤ i ⇒ ¬EL j bL2) ∧ bL1 = GENLIST (λn. n = i) (LENGTH vL) ∧
-     v1 ∉ freevars x1 ∧ EVERY (λv. v ∉ freevars x1) vL ∧
+[~Let_Lams_combine1:]
+  (∀v1 v2 vL1 vL2 vL3 bL1 bL2 bL3 x1 x2 y1 y2 i.
+     LENGTH vL1 = LENGTH bL2 ∧ LENGTH vL1 = LENGTH vL2 ∧ LENGTH vL1 = LENGTH bL3 ∧
+     ¬MEM v1 vL1 ∧ ALL_DISTINCT vL1 ∧ vL1 ≠ [] ∧ ALL_DISTINCT (vL3 ++ vL2) ∧
+     (∀i. i < LENGTH vL1 ⇒ (EL i vL1 = EL i vL2 ⇔ ¬EL i bL2)) ∧
+     LIST_REL (λb3 b2. b3 ⇒ b2) bL3 bL2 ∧
+     vL3 = MAP SND (FILTER FST (ZIP (bL3, vL1))) ∧
+
+     i < LENGTH vL1 ∧ (∀j. j ≤ i ⇒ ¬EL j bL2) ∧ bL1 = GENLIST (λn. n = i) (LENGTH vL1) ∧
+     v1 ∉ freevars x1 ∧ EVERY (λv. v ∉ freevars x1) (vL1 ++ vL2 ++ vL3) ∧
+
      exp_rel x1 x2 ∧ exp_rel y1 y2 ∧ v1 ≠ v2 ⇒
-     exp_rel (Let (SOME v1) (Lams vL (Apps x1 (MAP2 (λb e. if b then Force e else e) bL1 (MAP Var vL))))
-              (Let (SOME v2) (Lams vL (Apps (Var v1) (MAP2 (λb e. if b then Force e else e) bL2 (MAP Var vL)))) y1))
-             (Let (SOME v1) (Lams vL (Apps x2 (MAP2 (λb e. if b then Force e else e) bL1 (MAP Var vL))))
-              (Let (SOME v2) (Lams vL (Tick (Apps x2
-                                             (MAP2 (λb e. if b then Force e else e) bL1
-                                              (MAP2 (λb e. if b then Force e else e) bL2 (MAP Var vL)))))) y2))) ∧
+     exp_rel (Let (SOME v1) (Lams (vL3 ++ vL2) (Apps x1 (MAP Var vL3 ++
+                                                         MAP2 (λb e. if b then Force e else e) bL1 (MAP Var vL2))))
+              (Let (SOME v2) (Lams vL1 (Apps (Var v1) (MAP Var vL3 ++
+                                                      MAP2 (λb e. if b then Force e else e) bL2 (MAP Var vL1)))) y1))
+             (Let (SOME v1) (Lams (vL3 ++ vL2) (Apps x2 (MAP Var vL3 ++
+                                                         MAP2 (λb e. if b then Force e else e) bL1 (MAP Var vL2))))
+              (Let (SOME v2) (Lams vL1 (Tick (Apps x2
+                                              (MAP Var vL3 ++
+                                               MAP2 (λb e. if b then Force e else e) bL1
+                                                (MAP2 (λb e. if b then Force e else e) bL2 (MAP Var vL1)))))) y2))) ∧
+[~Let_Lams_combine2:]
+  (∀v1 v2 vL1 vL2 vL3 bL1 bL2 bL3 x1 x2 y1 y2 i.
+     LENGTH vL1 = LENGTH bL2 ∧ LENGTH vL1 = LENGTH vL2 ∧ LENGTH vL1 = LENGTH bL3 ∧
+     ¬MEM v1 vL1 ∧ ALL_DISTINCT vL1 ∧ vL1 ≠ [] ∧ ALL_DISTINCT (vL3 ++ vL2) ∧
+     (∀i. i < LENGTH vL1 ⇒ (EL i vL1 = EL i vL2 ⇔ ¬EL i bL2)) ∧
+     LIST_REL (λb3 b2. b3 ⇒ b2) bL3 bL2 ∧
+     vL3 = MAP SND (FILTER FST (ZIP (bL3, vL1))) ∧
+
+     i < LENGTH vL1 ∧ (∀j. j ≤ i ⇒ ¬EL j bL2) ∧ bL1 = GENLIST (λn. n = i) (LENGTH vL1) ∧
+     v1 ∉ freevars x1 ∧ EVERY (λv. v ∉ freevars x1) (vL1 ++ vL2 ++ vL3) ∧
+
+     exp_rel x1 x2 ∧ exp_rel y1 y2 ∧ v1 ≠ v2 ⇒
+     exp_rel (Let (SOME v1) (Lams (vL3 ++ vL2) (Apps x1 (Var (EL i vL2)::MAP Var vL3 ++
+                                                         MAP2 (λb e. if b then Force e else e) bL1 (MAP Var vL2))))
+              (Let (SOME v2) (Lams vL1 (Apps (Var v1)(MAP Var vL3 ++
+                                                      MAP2 (λb e. if b then Force e else e) bL2 (MAP Var vL1)))) y1))
+             (Let (SOME v1) (Lams (vL3 ++ vL2) (Apps x2 (Var (EL i vL2)::
+                                                         MAP Var vL3 ++
+                                                         MAP2 (λb e. if b then Force e else e) bL1 (MAP Var vL2))))
+              (Let (SOME v2) (Lams vL1 (Tick (Apps x2
+                                              (Var (EL i vL1)::
+                                               MAP Var vL3 ++
+                                               MAP2 (λb e. if b then Force e else e) bL1
+                                                (MAP2 (λb e. if b then Force e else e) bL2 (MAP Var vL1)))))) y2))) ∧
 [~If:]
   (∀x1 y1 z1 x2 y2 z2.
      exp_rel x1 x2 ∧
@@ -90,24 +123,39 @@ Inductive exp_rel:
   (∀s x y.
      exp_rel x y ⇒
        v_rel (Closure s x) (Closure s y)) ∧
-[v_rel_Closure_combine:]
-  (∀vL1 vL2 eL1 eL2 bL1 bL2 x y i.
-     LENGTH vL1 = LENGTH eL1 ∧ vL2 ≠ [] ∧ LENGTH (vL1 ++ vL2)  = LENGTH bL2 ∧
-     ALL_DISTINCT (vL1 ++ vL2) ∧
+[v_rel_Closure_combine1:]
+  (∀vL1a vL1b vL2 vL3a vL3b eL1a eL1 eL2a eL2 bL1 bL2 bL3a bL3b x y i.
+     LENGTH (vL1a ++ vL1b) = LENGTH vL2 ∧
+     LENGTH vL1a = LENGTH eL1 ∧ vL1b ≠ [] ∧ LENGTH (vL1a ++ vL1b)  = LENGTH bL2 ∧
+     ALL_DISTINCT (vL1a ++ vL1b) ∧ ALL_DISTINCT (vL3a ++ vL3b ++ vL2) ∧
+     LENGTH bL3a = LENGTH vL1a ∧ LENGTH bL3b = LENGTH vL1b ∧
+     LENGTH eL1a = LENGTH vL3a ∧
+     (∀i. i < LENGTH vL2 ⇒ (EL i (vL1a ++ vL1b) = EL i vL2 ⇔ ¬EL i bL2)) ∧
+     eL1a = MAP SND (FILTER FST (ZIP (bL3a, eL1))) ∧
+     eL2a = MAP SND (FILTER FST (ZIP (bL3a, eL2))) ∧
+     vL3a = MAP SND (FILTER FST (ZIP (bL3a, vL1a))) ∧
+     vL3b = MAP SND (FILTER FST (ZIP (bL3b, vL1b))) ∧
+     LIST_REL (λb3 b2. b3 ⇒ b2) (bL3a ++ bL3b) bL2 ∧
+
      LIST_REL v_rel eL1 eL2 ∧
      i < LENGTH bL2 ∧ (∀j. j ≤ i ⇒ ¬EL j bL2) ∧ bL1 = GENLIST (λn. n = i) (LENGTH bL2) ∧
-     EVERY (λv. v ∉ freevars x) (vL1 ++ vL2) ∧
+     EVERY (λv. v ∉ freevars x) (vL1a ++ vL1b ++ vL2 ++ vL3a ++ vL3b) ∧
      exp_rel x y ⇒
-     v_rel (Closure (HD vL2)
-            (Lams (TL vL2) (Apps (Value (
-                                   Closure (HD (vL1 ++ vL2))
-                                   (Lams (TL (vL1 ++ vL2)) (Apps x (MAP2 (λb e. if b then Force e else e)
-                                                                    bL1 (MAP Var (vL1 ++ vL2)))))))
-                            (MAP2 (λb e. if b then Force e else e) bL2 (MAP Value eL1 ++ MAP Var vL2)))))
-           (Closure (HD vL2)
-            (Lams (TL vL2) (Tick (Apps y
-                                  (MAP2 (λb e. if b then Force e else e) bL1
-                                   (MAP2 (λb e. if b then Force e else e) bL2 (MAP Value eL2 ++ MAP Var vL2)))))))) ∧
+     v_rel (Closure (HD vL1b)
+            (Lams (TL vL1b) (Apps (Value (
+                                   Closure (HD (vL3a ++ vL3b ++ vL2))
+                                   (Lams (TL (vL3a ++ vL3b ++ vL2))
+                                    (Apps x (MAP Var vL3a ++ MAP Var vL3b ++
+                                             MAP2 (λb e. if b then Force e else e)
+                                                  bL1 (MAP Var vL2))))))
+                             (MAP Value eL1a ++ MAP Var vL3b ++
+                                  MAP2 (λb e. if b then Force e else e) bL2 (MAP Value eL1 ++ MAP Var vL1b)))))
+           (Closure (HD vL1b)
+            (Lams (TL vL1b)(Tick(Apps y
+                                 (MAP Value eL2a ++ MAP Var vL3b ++
+                                  MAP2 (λb e. if b then Force e else e) bL1
+                                       (MAP2 (λb e. if b then Force e else e) bL2
+                                        (MAP Value eL2 ++ MAP Var vL1b)))))))) ∧
 [v_rel_Recclosure:]
   (∀f g n.
      MAP FST f = MAP FST g ∧
@@ -177,19 +225,41 @@ Proof
   >~[‘Let opt _ _’]
   >- (Cases_on ‘opt’ >> gvs [freevars_def])
   >- (gvs [freevars_Lams, freevars_def, freevars_Apps] >>
-      rw [SET_EQ_SUBSET, SUBSET_DEF]
-      >- (disj2_tac \\ disj1_tac \\ gs [] \\ disj2_tac
-          \\ gvs [MEM_EL, EL_MAP, EL_MAP2, PULL_EXISTS, SF CONJ_ss]
-          \\ first_assum $ irule_at Any \\ gvs [LIST_REL_EL_EQN]
-          \\ Cases_on ‘EL n bL2’ \\ gvs [freevars_def])
-      >- gvs []
-      >- gvs []
+      rw [SET_EQ_SUBSET, SUBSET_DEF] \\ gvs []
+      >- (gvs [MEM_MAP, MEM_FILTER, freevars_def]
+          \\ gvs [MEM_EL, EL_ZIP])
+      >- (gvs [MEM_EL, EL_MAP, EL_MAP2]
+          \\ rename1 ‘n < _’ \\ Cases_on ‘EL n bL2’
+          \\ gvs [freevars_def])
+      >- (disj1_tac \\ conj_tac \\ strip_tac
+          \\ gvs [EVERY_MEM, MEM_MAP, MEM_FILTER]
+          \\ gvs [MEM_EL, EL_ZIP])
+      >- (gvs [MEM_MAP, MEM_FILTER, freevars_def]
+          \\ gvs [MEM_EL, EL_ZIP])
       >- (gvs [MEM_EL, EL_MAP, EL_MAP2, PULL_EXISTS, SF CONJ_ss, LIST_REL_EL_EQN,
                freevars_def]
           \\ qpat_x_assum ‘_ ∈ freevars _’ mp_tac
           \\ IF_CASES_TAC >- (strip_tac \\ gvs [freevars_def])
-          \\ IF_CASES_TAC \\ strip_tac \\ gvs [freevars_def])
-      >- gvs [])
+          \\ IF_CASES_TAC \\ strip_tac \\ gvs [freevars_def]))
+  >- (gvs [freevars_Lams, freevars_def, freevars_Apps] >>
+      rw [SET_EQ_SUBSET, SUBSET_DEF] \\ gvs []
+      >- (gvs [MEM_MAP, MEM_FILTER, freevars_def]
+          \\ gvs [MEM_EL, EL_ZIP])
+      >- (gvs [MEM_EL, EL_MAP, EL_MAP2]
+          \\ rename1 ‘n < _’ \\ Cases_on ‘EL n bL2’
+          \\ gvs [freevars_def])
+      >- (disj1_tac \\ conj_tac \\ strip_tac
+          \\ gvs [EVERY_MEM, MEM_MAP, MEM_FILTER]
+          \\ gvs [MEM_EL, EL_ZIP])
+      >- (gvs [MEM_MAP, MEM_FILTER, freevars_def]
+          \\ gvs [MEM_EL, EL_ZIP])
+      >- (gvs [MEM_MAP, MEM_FILTER, freevars_def]
+          \\ gvs [MEM_EL, EL_ZIP])
+      >- (gvs [MEM_EL, EL_MAP, EL_MAP2, PULL_EXISTS, SF CONJ_ss, LIST_REL_EL_EQN,
+               freevars_def]
+          \\ qpat_x_assum ‘_ ∈ freevars _’ mp_tac
+          \\ IF_CASES_TAC >- (strip_tac \\ gvs [freevars_def])
+          \\ IF_CASES_TAC \\ strip_tac \\ gvs [freevars_def]))
 QED
 
 Theorem LIST_FILTERED:
@@ -266,43 +336,123 @@ Proof
     \\ gvs [MAP_FST_FILTER, LAMBDA_PROD]
     \\ irule LIST_REL_FILTER
     \\ gvs [LIST_REL_EL_EQN])
-  >~[‘Let _ _ (Let _ _ _)’]
-  >- (gvs [subst_def, subst_Lams, subst_Apps]
-      \\ gvs [exp_rel_def] \\ disj2_tac
+  >~[‘Apps (App _ _) _’]
+  >- (gvs [subst_def, subst_Lams, subst_Apps, GSYM LAMBDA_PROD, FILTER_T,
+           GSYM FILTER_REVERSE, ALOOKUP_FILTER, EL_MEM]
+      \\ gvs [exp_rel_def] \\ disj2_tac \\ disj2_tac
       \\ rpt (‘∀l1 l2 e1 e2. l1 = l2 ∧ e1 = e2 ⇒ Lams l1 e1 = Lams l2 e2’ by gs []
               \\ pop_assum $ irule_at Any)
       \\ gvs []
       \\ rpt (‘∀l1 l2 e1 e2. l1 = l2 ∧ e1 = e2 ⇒ Apps e1 l1 = Apps e2 l2’ by gs []
               \\ pop_assum $ irule_at Any)
       \\ gvs []
-      \\ rename1 ‘i < LENGTH bL2’ \\ qexists_tac ‘i’
-      \\ qexists_tac ‘bL2’ \\ rw []
-      >- (irule LIST_EQ \\ rw [EL_MAP, EL_MAP2]
-          \\ gvs [subst_def, GSYM FILTER_REVERSE, ALOOKUP_FILTER, EL_MEM])
-      >- (irule LIST_EQ \\ rw [EL_MAP, EL_MAP2]
-          \\ gvs [subst_def, GSYM FILTER_REVERSE, ALOOKUP_FILTER, EL_MEM])
-      >- gvs [GSYM FILTER_REVERSE, ALOOKUP_FILTER]
-      >- (irule LIST_EQ \\ rw [EL_MAP, EL_MAP2]
-          \\ gvs [subst_def, GSYM FILTER_REVERSE, ALOOKUP_FILTER, EL_MEM])
-      >- (irule LIST_EQ \\ rw [EL_MAP, EL_MAP2]
-          \\ gvs [subst_def, GSYM FILTER_REVERSE, ALOOKUP_FILTER, EL_MEM])
+      \\ irule_at (Pos $ el 2) EQ_REFL
+      \\ rpt (‘∀l1 l2 e1 (e2 : exp list). l1 = l2 ∧ e1 = e2 ⇒ e1 ++ l1 = e2 ++ l2’ by gs []
+              \\ pop_assum $ irule_at Any)
+      \\ gvs [SF CONJ_ss]
+      \\ qexists_tac ‘bL3’ \\ qexists_tac ‘bL2’ \\ rw []
+      >- (irule LIST_EQ \\ rw [EL_MAP, EL_MAP2, subst_def, GSYM FILTER_REVERSE, ALOOKUP_FILTER, EL_MEM])
+      >- (irule LIST_EQ \\ rw [EL_MAP, EL_MAP2, subst_def, GSYM FILTER_REVERSE, ALOOKUP_FILTER, EL_MEM]
+          \\ dxrule_then assume_tac EL_MEM
+          \\ gvs [MEM_FILTER] \\ gvs [MEM_EL, EL_ZIP])
+      >- (irule LIST_EQ \\ rw [EL_MAP, EL_MAP2, subst_def, GSYM FILTER_REVERSE, ALOOKUP_FILTER, EL_MEM])
+      >- (irule LIST_EQ \\ rw [EL_MAP, EL_MAP2, subst_def, GSYM FILTER_REVERSE, ALOOKUP_FILTER, EL_MEM]
+          \\ gvs [MEM_MAP]
+          \\ first_x_assum $ resolve_then (Pos hd) assume_tac EQ_REFL
+          \\ gvs [EL_MEM])
+      >- (irule LIST_EQ \\ rw [EL_MAP, EL_MAP2, subst_def, GSYM FILTER_REVERSE, ALOOKUP_FILTER, EL_MEM])
+      >- (irule LIST_EQ \\ rw [EL_MAP, EL_MAP2, subst_def, GSYM FILTER_REVERSE, ALOOKUP_FILTER, EL_MEM]
+          \\ dxrule_then assume_tac EL_MEM
+          \\ gvs [MEM_FILTER] \\ gvs [MEM_EL, EL_ZIP])
+      >- (irule LIST_EQ \\ rw [EL_MAP, EL_MAP2, subst_def, GSYM FILTER_REVERSE, ALOOKUP_FILTER, EL_MEM])
+      >- (irule LIST_EQ \\ rw [EL_MAP, EL_MAP2, subst_def, GSYM FILTER_REVERSE, ALOOKUP_FILTER, EL_MEM]
+          \\ gvs [MEM_MAP]
+          \\ first_x_assum $ resolve_then (Pos hd) assume_tac EQ_REFL
+          \\ gvs [EL_MEM])
       >- (gvs [FILTER_FILTER, LAMBDA_PROD]
-          \\ rename1 ‘subst (FILTER _ ws) y’
-          \\ qspecl_then [‘FILTER (λ(p1, p2). ¬MEM p1 vL) ws’, ‘y’, ‘{v1}’]
-                         assume_tac subst_remove
+          \\ rename1 ‘subst (FILTER (λ(p1, p2). ¬MEM p1 vL1 ∧ p1 ≠ v1) ws) y = subst (FILTER _ ws) _’
+          \\ qspecl_then [‘ws’, ‘y’, ‘set vL1 ∪ {v1}’] mp_tac subst_remove \\ impl_tac \\ gvs []
+          >- (qspecl_then [‘x’, ‘y’] assume_tac exp_rel_freevars
+              \\ gvs [DISJOINT_ALT, EVERY_MEM])
+          \\ disch_then kall_tac
+          \\ qspecl_then [‘ws’, ‘y’, ‘set (MAP SND (FILTER FST (ZIP (bL3, vL1)))) ∪ set vL2’] mp_tac
+                         $ GSYM subst_remove
+          \\ impl_tac \\ gvs []
           \\ qspecl_then [‘x’, ‘y’] assume_tac exp_rel_freevars
-          \\ gvs [FILTER_FILTER, LAMBDA_PROD]
-          \\ irule EQ_TRANS \\ first_x_assum $ irule_at Any
-          \\ AP_THM_TAC \\ AP_TERM_TAC \\ AP_THM_TAC \\ AP_TERM_TAC \\ gvs [CONJ_COMM])
+          \\ gvs [DISJOINT_ALT, EVERY_MEM])
       >- gvs [freevars_subst]
       >- gvs [EVERY_MEM, freevars_subst]
-      \\ first_x_assum irule \\ gvs [MAP_FST_FILTER, EVERY2_MAP, FILTER_FILTER, LAMBDA_PROD]
-      >- (qabbrev_tac ‘P = λn. ¬MEM n vL’ \\ gs [] \\ irule LIST_REL_FILTER \\ gs []
+      >- gvs [EVERY_MEM, freevars_subst]
+      >- gvs [EVERY_MEM, freevars_subst]
+      >- (first_x_assum irule \\ gvs [MAP_FST_FILTER, EVERY2_MAP]
+          \\ qabbrev_tac ‘P = λv. ¬MEM v (MAP SND (FILTER FST (ZIP (bL3, vL1)))) ∧ ¬MEM v vL2’ \\ gvs []
+          \\ irule LIST_REL_FILTER \\ gs []
           \\ irule LIST_REL_mono
-          \\ first_x_assum $ irule_at Any \\ gvs [])
-      \\ qabbrev_tac ‘P = λn. n ≠ v2 ∧ n ≠ v1’ \\ gs [] \\ irule LIST_REL_FILTER \\ gs []
-      \\ irule LIST_REL_mono
-      \\ first_x_assum $ irule_at Any \\ gvs [])
+          \\ first_x_assum $ irule_at $ Pos last
+          \\ gvs [])
+      >- (first_x_assum irule \\ gvs [MAP_FST_FILTER, EVERY2_MAP, FILTER_FILTER, LAMBDA_PROD]
+          \\ qabbrev_tac ‘P = λv. v ≠ v2 ∧ v ≠ v1’ \\ gvs []
+          \\ irule LIST_REL_FILTER \\ gs []
+          \\ irule LIST_REL_mono
+          \\ first_x_assum $ irule_at $ Pos last
+          \\ gvs []))
+  >~[‘Let _ _ (Let _ _ _)’]
+  >- (gvs [subst_def, subst_Lams, subst_Apps, GSYM LAMBDA_PROD, FILTER_T,
+           GSYM FILTER_REVERSE, ALOOKUP_FILTER, EL_MEM]
+      \\ gvs [exp_rel_def] \\ disj2_tac \\ disj1_tac
+      \\ rpt (‘∀l1 l2 e1 e2. l1 = l2 ∧ e1 = e2 ⇒ Lams l1 e1 = Lams l2 e2’ by gs []
+              \\ pop_assum $ irule_at Any)
+      \\ gvs []
+      \\ rpt (‘∀l1 l2 e1 e2. l1 = l2 ∧ e1 = e2 ⇒ Apps e1 l1 = Apps e2 l2’ by gs []
+              \\ pop_assum $ irule_at Any)
+      \\ gvs []
+      \\ qpat_assum ‘_ < LENGTH _’ $ irule_at Any
+      \\ qpat_assum ‘LIST_REL (λb3 b2. b3 ⇒ b2) _ _’ $ irule_at Any
+      \\ gvs [EVERY_MEM, freevars_subst]
+      \\ rpt (‘∀l1 l2 e1 (e2 : exp list). l1 = l2 ∧ e1 = e2 ⇒ e1 ++ l1 = e2 ++ l2’ by gs []
+              \\ pop_assum $ irule_at Any)
+      \\ rw []
+      >- (irule LIST_EQ \\ rw [EL_MAP, EL_MAP2, subst_def, GSYM FILTER_REVERSE, ALOOKUP_FILTER, EL_MEM])
+      >- (irule LIST_EQ \\ rw [EL_MAP, EL_MAP2, subst_def, GSYM FILTER_REVERSE, ALOOKUP_FILTER, EL_MEM]
+          \\ dxrule_then assume_tac EL_MEM
+          \\ gvs [MEM_FILTER] \\ gvs [MEM_EL, EL_ZIP])
+      >- (irule LIST_EQ \\ rw [EL_MAP, EL_MAP2, subst_def, GSYM FILTER_REVERSE, ALOOKUP_FILTER, EL_MEM])
+      >- (irule LIST_EQ \\ rw [EL_MAP, EL_MAP2, subst_def, GSYM FILTER_REVERSE, ALOOKUP_FILTER, EL_MEM]
+          \\ gvs [MEM_MAP]
+          \\ first_x_assum $ resolve_then (Pos hd) assume_tac EQ_REFL
+          \\ gvs [EL_MEM])
+      >- (irule LIST_EQ \\ rw [EL_MAP, EL_MAP2, subst_def, GSYM FILTER_REVERSE, ALOOKUP_FILTER, EL_MEM])
+      >- (irule LIST_EQ \\ rw [EL_MAP, EL_MAP2, subst_def, GSYM FILTER_REVERSE, ALOOKUP_FILTER, EL_MEM]
+          \\ dxrule_then assume_tac EL_MEM
+          \\ gvs [MEM_FILTER] \\ gvs [MEM_EL, EL_ZIP])
+      >- (irule LIST_EQ \\ rw [EL_MAP, EL_MAP2, subst_def, GSYM FILTER_REVERSE, ALOOKUP_FILTER, EL_MEM])
+      >- (irule LIST_EQ \\ rw [EL_MAP, EL_MAP2, subst_def, GSYM FILTER_REVERSE, ALOOKUP_FILTER, EL_MEM]
+          \\ gvs [MEM_MAP]
+          \\ first_x_assum $ resolve_then (Pos hd) assume_tac EQ_REFL
+          \\ gvs [EL_MEM])
+      >- (gvs [FILTER_FILTER, LAMBDA_PROD]
+          \\ rename1 ‘subst (FILTER (λ(p1, p2). ¬MEM p1 vL1 ∧ p1 ≠ v1) ws) y = subst (FILTER _ ws) _’
+          \\ qspecl_then [‘ws’, ‘y’, ‘set vL1 ∪ {v1}’] mp_tac subst_remove \\ impl_tac \\ gvs []
+          >- (qspecl_then [‘x’, ‘y’] assume_tac exp_rel_freevars
+              \\ gvs [DISJOINT_ALT, EVERY_MEM])
+          \\ disch_then kall_tac
+          \\ qspecl_then [‘ws’, ‘y’, ‘set (MAP SND (FILTER FST (ZIP (bL3, vL1)))) ∪ set vL2’] mp_tac
+                         $ GSYM subst_remove
+          \\ impl_tac \\ gvs []
+          \\ qspecl_then [‘x’, ‘y’] assume_tac exp_rel_freevars
+          \\ gvs [DISJOINT_ALT, EVERY_MEM])
+      >- (first_x_assum irule \\ gvs [MAP_FST_FILTER, EVERY2_MAP]
+          \\ qabbrev_tac ‘P = λv. ¬MEM v (MAP SND (FILTER FST (ZIP (bL3, vL1)))) ∧ ¬MEM v vL2’ \\ gvs []
+          \\ irule LIST_REL_FILTER \\ gs []
+          \\ irule LIST_REL_mono
+          \\ first_x_assum $ irule_at $ Pos last
+          \\ gvs [])
+      >- (first_x_assum irule \\ gvs [MAP_FST_FILTER, EVERY2_MAP, FILTER_FILTER, LAMBDA_PROD]
+          \\ qabbrev_tac ‘P = λv. v ≠ v2 ∧ v ≠ v1’ \\ gvs []
+          \\ irule LIST_REL_FILTER \\ gs []
+          \\ irule LIST_REL_mono
+          \\ first_x_assum $ irule_at $ Pos last
+          \\ gvs [FORALL_PROD]))
   >~ [‘Let s x y’] >- (
     Cases_on ‘s’ \\ rw [subst_def]
     \\ irule exp_rel_Let \\ gs []
@@ -818,6 +968,7 @@ Proof
         \\ dxrule_then (qspecl_then [‘j + j1 + j2 + k - 1’] assume_tac) eval_to_mono
         \\ gvs [])
 
+    (* combine closure1 *)
     >- (IF_CASES_TAC \\ gvs []
         >- (qexists_tac ‘0’ \\ gvs []
             \\ Cases_on ‘eval_to 0 y = INL Diverge’ \\ gs []
@@ -825,20 +976,33 @@ Proof
             \\ Cases_on ‘eval_to 0 g = INL Diverge’ \\ gs []
             \\ dxrule_then (qspecl_then [‘j1’] assume_tac) eval_to_mono
             \\ gvs [])
-        \\ Cases_on ‘vL2’ \\ gs []
-        \\ rename1 ‘Lams vL2 _’ \\ Cases_on ‘vL2 = []’ \\ gvs []
+        \\ Cases_on ‘vL1b’ \\ gs []
+        \\ Cases_on ‘bL3b’ \\ gs []
+        \\ rename1  ‘LIST_REL _ (bL3a ++ b::bL3b) bL2’
+        \\ rename1 ‘eval_to _ (subst1 h v1 (Lams vL1b _))’ \\ Cases_on ‘vL1b = []’ \\ gvs []
         >- (gvs [subst_Apps, subst1_def]
-            \\ ‘MAP (subst [(h,v1)]) (MAP2 (λb e. if b then Force e else e) bL2 (MAP Value eL1 ++ [Var h]))
+            \\ ‘MAP (subst [(h,v1)])
+                (MAP Value (MAP SND (FILTER FST (ZIP (bL3a,eL1)))))
+                = MAP Value (MAP SND (FILTER FST (ZIP (bL3a,eL1))))’
+              by (irule LIST_EQ \\ gvs [EL_MAP, EL_MAP2, subst1_def])
+            \\ gs [] \\ pop_assum kall_tac
+            \\ ‘MAP (subst [(h,v1)])
+                (MAP2 (λb e. if b then Force e else e) bL2 (MAP Value eL1 ++ [Var h]))
                 = MAP2 (λb e. if b then Force e else e) bL2 (MAP Value eL1 ++ [Value v1])’
-              by (irule LIST_EQ \\ gvs [LIST_REL_EL_EQN] \\ rw [EL_MAP, EL_MAP2, EL_APPEND_EQN, subst1_def]
-                  \\ gvs [NOT_LESS] \\ Cases_on ‘LENGTH bL2’ \\ gvs [GSYM ADD1, GSYM LESS_EQ_IFF_LESS_SUC]
-                  \\ dxrule_then (dxrule_then assume_tac) LESS_EQUAL_ANTISYM
-                  \\ gvs [subst1_def])
-            \\ gvs [] \\ pop_assum kall_tac
+              by (irule LIST_EQ \\ gvs [EL_MAP, EL_MAP2, subst1_def]
+                  \\ rw [subst_def, EL_APPEND_EQN, EL_MAP]
+                  \\ Cases_on ‘LENGTH vL2’ \\ gvs [NOT_LESS, GSYM ADD1, GSYM LESS_EQ_IFF_LESS_SUC]
+                  \\ dxrule_then assume_tac LESS_EQUAL_ANTISYM \\ gs [subst1_def])
+            \\ gs [] \\ pop_assum kall_tac
+            \\ ‘MAP (subst [(h,v1)]) (MAP Var (MAP SND (if b then [(T,h)] else [])))
+                = if b then [Value v1] else []’
+              by (IF_CASES_TAC \\ gvs [subst_def])
+            \\ gs [] \\ pop_assum kall_tac
             \\ Cases_on ‘∃i. i < SUC (LENGTH eL1) ∧ eval_to (k - 1) (EL i (MAP2 (λb e. if b then Force e else e)
                                                                      bL2 (MAP Value eL1 ++ [Value v1])))
                                                     = INL Diverge’ \\ gvs []
             >- (rename1 ‘eval_to _ (EL i2 _) = INL Diverge’
+                \\ gvs [FOLDL_APPEND]
                 \\ qmatch_goalsub_abbrev_tac ‘($= +++ v_rel) (eval_to _ (Apps expr1 argL1)) _’
                 \\ qspecl_then [‘argL1’, ‘i2’, ‘k - 1’, ‘expr1’] mp_tac eval_to_Apps_arg_Div \\ gvs []
                 \\ impl_tac >- gvs [Abbr ‘argL1’] \\ rw []
@@ -852,8 +1016,8 @@ Proof
                 \\ Cases_on ‘k = 1’
                 \\ gvs [subst_Apps, subst1_notin_frees, freevars_def, subst1_def, eval_to_Tick]
                 >- simp [eval_to_def]
-                \\ qmatch_goalsub_abbrev_tac ‘($= +++ v_rel) _ (eval_to _ (Apps _ argL2))’
-                \\ qspecl_then [‘argL1’, ‘argL2’, ‘i2’, ‘k - 2’, ‘expr1’, ‘y2’]
+                \\ qmatch_goalsub_abbrev_tac ‘($= +++ v_rel) _ (eval_to _ (Apps expr2 argL2))’
+                \\ qspecl_then [‘argL1’, ‘argL2’, ‘i2’, ‘k - 2’, ‘expr1’, ‘expr2’]
                                mp_tac eval_to_Apps_arg_Div_exp_rel
                 \\ impl_tac \\ gvs []
                 \\ conj_tac
@@ -882,55 +1046,103 @@ Proof
                 \\ first_x_assum irule
                 \\ IF_CASES_TAC \\ gvs [EL_APPEND_EQN, EL_MAP, subst1_def]
                 \\ IF_CASES_TAC \\ gvs [exp_rel_def, subst1_def]
-                \\ Cases_on ‘LENGTH bL2’ \\ gvs []
+                \\ Cases_on ‘LENGTH vL2’ \\ gvs []
                 \\ gvs [NOT_LESS, GSYM LESS_EQ_IFF_LESS_SUC, GSYM ADD1]
                 \\ dxrule_then (dxrule_then assume_tac) LESS_EQUAL_ANTISYM
                 \\ gvs [subst1_def, exp_rel_def])
+            \\ gvs [FOLDL_APPEND]
             \\ qmatch_goalsub_abbrev_tac ‘($= +++ v_rel) (eval_to _ (Apps expr1 argL1)) _’
             \\ qspecl_then [‘argL1’, ‘expr1’, ‘k - 1’] mp_tac eval_to_Apps_no_INL
             \\ gvs [] \\ impl_tac
             >- (rw [] \\ strip_tac \\ first_x_assum $ dxrule_then assume_tac \\ gvs [Abbr ‘argL1’])
             \\ disch_then $ qx_choose_then ‘valL1’ assume_tac \\ gvs [Abbr ‘expr1’]
+            \\ pop_assum kall_tac
+            \\ ‘LENGTH vL2 = LENGTH valL1’ by gvs [Abbr ‘argL1’, LIST_REL_EL_EQN]
             \\ Cases_on ‘k - 1 = 0’ \\ gvs []
             >- (dxrule_then assume_tac LESS_EQ_CASES \\ gvs []
-                \\ ‘LENGTH bL2 = LENGTH valL1’ by gvs [Abbr ‘argL1’, LIST_REL_EL_EQN]
-                \\ qspecl_then [‘vL1 ++ [h]’, ‘valL1’] assume_tac eval_to_Apps_Lams_0 \\ gvs []
+                \\ qspecl_then [‘(MAP SND (FILTER FST (ZIP (bL3a,vL1a))) ++
+                                  MAP SND (if b then [(T,h)] else []) ++ vL2)’,
+                                ‘MAP SND (FILTER FST (ZIP (bL3a,eL1)))
+                                 ++ (if b then [v1] else []) ++ valL1’] assume_tac eval_to_Apps_Lams_0
+                \\ gvs [FOLDL_APPEND]
+                \\ ‘MAP Value (if b then [v1] else []) = if b then [Value v1] else []’ by (IF_CASES_TAC \\ gs [])
+                \\ gvs []
+                \\ Cases_on ‘vL2 = []’ \\ gs []
+                \\ Cases_on ‘b’ \\ gvs []
                 \\ qexists_tac ‘0’
                 \\ Cases_on ‘eval_to 1 y = INL Diverge’ \\ gs []
                 \\ dxrule_then assume_tac eval_to_mono \\ gs []
                 \\ Cases_on ‘eval_to 1 g = INL Diverge’ \\ gs []
                 \\ dxrule_then assume_tac eval_to_mono \\ gs []
                 \\ gvs [subst1_def, eval_to_def])
-            \\ ‘LENGTH bL2 = LENGTH valL1’ by gvs [Abbr ‘argL1’, LIST_REL_EL_EQN]
-            \\ qspecl_then [‘vL1 ++ [h]’, ‘valL1’] assume_tac eval_to_Apps_Lams_not_0 \\ gvs []
+            \\ ‘∀(v : thunkLang$v). MAP Value (if b then [v] else []) = if b then [Value v] else []’ by rw []
+            \\ ‘∀(h : string). LENGTH (if b then [(T, h)] else []) = if b then 1 else 0’ by rw []
+            \\ ‘∀(v : thunkLang$v). LENGTH (if b then [v] else []) = if b then 1 else 0’ by rw []
+            \\ Cases_on ‘vL2 = []’ \\ gvs []
+            \\ qspecl_then [‘MAP SND (FILTER FST (ZIP (bL3a,vL1a))) ++
+                             MAP SND (if b then [(T,h)] else []) ++ vL2’,
+                            ‘MAP SND (FILTER FST (ZIP (bL3a, eL1))) ++
+                             (if b then [v1] else []) ++ valL1’] assume_tac eval_to_Apps_Lams_not_0
+            \\ gvs [FOLDL_APPEND]
             \\ pop_assum kall_tac
-            \\ rename1 ‘subst _ (Apps x2 _)’
-            \\ qspecl_then [‘ZIP (vL1 ++ [h], valL1)’, ‘x2’] mp_tac subst_notin_frees
+            \\ rename1 ‘subst _ (Apps (Apps (Apps x2 _) _) _)’
+            \\ qmatch_goalsub_abbrev_tac ‘eval_to _ (subst list (Apps (Apps (Apps _ _) _) _))’
+            \\ qspecl_then [‘list’, ‘x2’] mp_tac subst_notin_frees
             \\ gvs [MAP_ZIP, DISJOINT_ALT] \\ impl_tac
-            >- (rw [] \\ gvs [EVERY_MEM])
+            >- (gvs [Abbr ‘list’, MAP_ZIP] \\ rw [] \\ gvs [EVERY_MEM])
             \\ strip_tac \\ gvs [subst_Apps] \\ pop_assum kall_tac
-            \\ ‘MAP (subst (ZIP (vL1 ++ [h],valL1))) (MAP2 (λb e. if b then Force e else e)
-                                                      (GENLIST (λn. n = i) (LENGTH valL1)) (MAP Var vL1 ++ [Var h]))
-                = MAP2 (λb e. if b then Force e else e) (GENLIST (λn. n = i) (LENGTH valL1)) (MAP Value valL1)’
-              by (irule LIST_EQ \\ gvs [EL_MAP2, EL_MAP] \\ rw [subst_def]
-                  >- (rw [EL_APPEND_EQN, EL_MAP, subst_def]
-                      >- (rename1 ‘i < _’
-                          \\ qspec_then ‘ZIP (vL1 ++ [h], valL1)’ assume_tac alookup_distinct_reverse
-                          \\ qspecl_then [‘ZIP (vL1 ++ [h], valL1)’, ‘i’] assume_tac ALOOKUP_ALL_DISTINCT_EL
-                          \\ gvs [ALL_DISTINCT_APPEND, MAP_ZIP, EL_ZIP, EL_APPEND_EQN])
-                      \\ qspec_then ‘valL1’ assume_tac SNOC_CASES \\ gs []
-                      \\ gvs [NOT_LESS, GSYM ADD1, GSYM ZIP_APPEND, GSYM LESS_EQ_IFF_LESS_SUC]
-                      \\ dxrule_then (dxrule_then assume_tac) LESS_EQUAL_ANTISYM
-                      \\ gvs [subst_def, REVERSE_APPEND, EL_APPEND_EQN])
-                  \\ rw [EL_APPEND_EQN, EL_MAP, subst_def]
-                  >- (rename1 ‘i2 < _’
-                      \\ qspec_then ‘ZIP (vL1 ++ [h], valL1)’ assume_tac alookup_distinct_reverse
-                      \\ qspecl_then [‘ZIP (vL1 ++ [h], valL1)’, ‘i2’] assume_tac ALOOKUP_ALL_DISTINCT_EL
-                      \\ gvs [ALL_DISTINCT_APPEND, MAP_ZIP, EL_ZIP, EL_APPEND_EQN])
-                  \\ qspec_then ‘valL1’ assume_tac SNOC_CASES \\ gs []
-                  \\ gvs [NOT_LESS, GSYM ADD1, GSYM ZIP_APPEND, GSYM LESS_EQ_IFF_LESS_SUC]
-                  \\ dxrule_then (dxrule_then assume_tac) LESS_EQUAL_ANTISYM
-                  \\ gvs [subst_def, REVERSE_APPEND, EL_APPEND_EQN])
+            \\ ‘MAP (subst list) (MAP Var (MAP SND (FILTER FST (ZIP (bL3a, vL1a)))))
+                = MAP Value (MAP SND (FILTER FST (ZIP (bL3a, eL1))))’
+              by (gvs [Abbr ‘list’, GSYM ZIP_APPEND]
+                  \\ irule LIST_EQ \\ gvs [EL_MAP, subst_def, REVERSE_APPEND, ALOOKUP_APPEND]
+                  \\ gen_tac \\ strip_tac \\ rename1 ‘n < LENGTH (FILTER _ _)’
+                  \\ drule_then assume_tac EL_MEM \\ gvs [MEM_FILTER, MEM_EL, EL_ZIP]
+                  \\ qspecl_then [‘REVERSE (ZIP (vL2, valL1))’, ‘SND (EL n (FILTER FST (ZIP (bL3a, vL1a))))’]
+                                 mp_tac $ iffRL ALOOKUP_NONE
+                  \\ impl_tac \\ gvs []
+                  >- (gvs [ALL_DISTINCT_APPEND, MAP_REVERSE, MAP_ZIP]
+                      \\ first_x_assum irule
+                      \\ disj1_tac \\ gvs [MEM_MAP, MEM_FILTER]
+                      \\ gvs [MEM_EL, EL_ZIP, SF CONJ_ss, PULL_EXISTS]
+                      \\ irule_at (Pos hd) EQ_REFL \\ gvs [])
+                  \\ disch_then kall_tac
+                  \\ qspecl_then [‘REVERSE (ZIP (MAP SND (if b then [(T,h)] else []),
+                                                          if b then [v1] else []))’,
+                                  ‘SND (EL n (FILTER FST (ZIP (bL3a, vL1a))))’]
+                                 mp_tac $ iffRL ALOOKUP_NONE
+                  \\ impl_tac \\ gvs []
+                  >- (IF_CASES_TAC \\ gvs []
+                      \\ strip_tac \\ gvs [ALL_DISTINCT_APPEND, MEM_MAP, MEM_FILTER, EL_MEM])
+                  \\ disch_then kall_tac
+                  \\ ‘ALL_DISTINCT (MAP FST (ZIP (MAP SND (FILTER FST (ZIP (bL3a,vL1a))),
+                                                  MAP SND (FILTER FST (ZIP (bL3a,eL1))))))’
+                    by gvs [MAP_ZIP, ALL_DISTINCT_APPEND]
+                  \\ gvs [alookup_distinct_reverse]
+                  \\ qspecl_then [‘ZIP (MAP SND (FILTER FST (ZIP (bL3a,vL1a))),
+                                        MAP SND (FILTER FST (ZIP (bL3a,eL1))))’,
+                                  ‘n’] mp_tac ALOOKUP_ALL_DISTINCT_EL
+                  \\ gvs [EL_ZIP, EL_MAP])
+            \\ gvs [] \\ pop_assum kall_tac
+           \\ ‘MAP (subst list) (MAP2 (λb e. if b then Force e else e)
+                                 (GENLIST (λn. n = i) (LENGTH valL1)) (MAP Var vL2))
+                = MAP2 (λb e. if b then Force e else e)
+                       (GENLIST (λn. n = i) (LENGTH valL1)) (MAP Value valL1)’
+              by (gvs [Abbr ‘list’, GSYM ZIP_APPEND]
+                  \\ irule LIST_EQ \\ gvs [EL_MAP, EL_MAP2]
+                  \\ gen_tac \\ strip_tac \\ rename1 ‘n < LENGTH _’
+                  \\ qspecl_then [‘ZIP (vL2, valL1)’] assume_tac $ GEN_ALL alookup_distinct_reverse
+                  \\ qspecl_then [‘ZIP (vL2, valL1)’, ‘n’] assume_tac ALOOKUP_ALL_DISTINCT_EL
+                  \\ Cases_on ‘n = i’ \\ gvs [subst_def, REVERSE_APPEND, ALOOKUP_APPEND]
+                  \\ gvs [MAP_ZIP, ALL_DISTINCT_APPEND, EL_ZIP])
+            \\ gvs [] \\ pop_assum kall_tac
+            \\ ‘MAP (subst list) (MAP Var (MAP SND (if b then [(T, h)] else [])))
+                = if b then [Value v1] else []’
+               by (gvs [Abbr ‘list’, GSYM ZIP_APPEND]
+                   \\ irule LIST_EQ \\ gvs [EL_MAP, subst_def, REVERSE_APPEND, ALOOKUP_APPEND]
+                   \\ IF_CASES_TAC \\ gvs []
+                   \\ Cases \\ gvs []
+                   \\ qspecl_then [‘REVERSE (ZIP (vL2, valL1))’, ‘h’] assume_tac ALOOKUP_NONE
+                   \\ gvs [MAP_REVERSE, MAP_ZIP, ALL_DISTINCT_APPEND])
             \\ gvs [] \\ pop_assum kall_tac
             \\ Cases_on ‘eval_to (k - 2) (Force (Value (EL i valL1))) = INL Diverge’ \\ gvs []
             >- (dxrule_then (qspec_then ‘i’ assume_tac) eval_to_Apps_arg_Div
@@ -952,11 +1164,12 @@ Proof
                       \\ gvs [GSYM ADD1, GSYM LESS_EQ_IFF_LESS_SUC, NOT_LESS]
                       \\ dxrule_then (dxrule_then assume_tac) LESS_EQUAL_ANTISYM \\ gvs [subst1_def])
                 \\ gvs [] \\ pop_assum kall_tac
+                \\ qmatch_goalsub_abbrev_tac ‘_ (INL Diverge) (eval_to _ (Apps expr2 _))’
                 \\ qspecl_then [‘MAP2 (λb e. if b then Force e else e) (GENLIST (λn. n = i) (LENGTH valL1))
                                   (MAP2 (λb e. if b then Force e else e) bL2 (MAP Value eL1 ++ [Value v1]))’,
                               ‘MAP2 (λb e. if b then Force e else e) (GENLIST (λn. n = i) (LENGTH valL1))
                                   (MAP2 (λb e. if b then Force e else e) bL2 (MAP Value eL2 ++ [Value w1]))’,
-                                ‘i’, ‘k - 2’, ‘y2’] mp_tac eval_to_Apps_arg_Div_exp_rel2
+                                ‘i’, ‘k - 2’, ‘expr2’] mp_tac eval_to_Apps_arg_Div_exp_rel2
                 \\ impl_tac \\ gvs [EL_MAP2, EL_MAP, EL_APPEND_EQN]
                 \\ ‘LENGTH valL1 = SUC (LENGTH eL1)’ by gvs []
                 \\ ‘EL i (eL1 ++ [v1]) = EL i valL1’
@@ -1003,7 +1216,7 @@ Proof
                     \\ gvs [EL_MAP2, EL_MAP, EL_APPEND_EQN, LIST_REL_EL_EQN]
                     \\ pop_assum $ qspec_then ‘i’ assume_tac
                     \\ gvs [Abbr ‘argL1’, EL_APPEND_EQN, EL_MAP2, EL_MAP, exp_rel_def]
-                    \\ last_x_assum $ qspec_then ‘i’ assume_tac \\ gvs [])
+                    \\ rpt $ last_x_assum $ qspec_then ‘i’ assume_tac \\ gvs [])
                 >- (last_x_assum $ qspec_then ‘k - 2’ assume_tac \\ gvs []
                     \\ pop_assum irule
                     \\ qpat_x_assum ‘LIST_REL _ _ _’ assume_tac
@@ -1036,12 +1249,12 @@ Proof
                     \\ dxrule_then (dxrule_then assume_tac) LESS_EQUAL_ANTISYM
                     \\ first_x_assum $ qspec_then ‘LENGTH eL2’ assume_tac
                     \\ gvs [EL_APPEND_EQN, EL_MAP2, EL_MAP, exp_rel_def, eval_to_Value]))
-            \\ qmatch_goalsub_abbrev_tac ‘($= +++ v_rel) (eval_to _ (Apps _ argL2)) _’
-            \\ qspecl_then [‘argL2’, ‘x2’, ‘k - 2’] mp_tac eval_to_Apps_no_INL
+            \\ qmatch_goalsub_abbrev_tac ‘($= +++ v_rel) (eval_to _ (Apps expr1 argL2)) _’
+            \\ qspecl_then [‘argL2’, ‘expr1’, ‘k - 2’] mp_tac eval_to_Apps_no_INL
             \\ gvs [] \\ impl_tac
             >- (gvs [Abbr ‘argL2’, EL_MAP2, EL_MAP] \\ rw [eval_to_Value])
             \\ disch_then $ qx_choose_then ‘valL2’ assume_tac \\ gvs []
-            \\ Cases_on ‘eval_to (k - 2) (Apps x2 (MAP Value valL2)) = INL Diverge’ \\ gvs []
+            \\ Cases_on ‘eval_to (k - 2) (Apps expr1 (MAP Value valL2)) = INL Diverge’ \\ gvs []
             >- (qexists_tac ‘0’
                 \\ Cases_on ‘eval_to k y = INL Diverge’ \\ gs []
                 \\ dxrule_then assume_tac eval_to_mono \\ gvs [] \\ pop_assum kall_tac
@@ -1109,17 +1322,29 @@ Proof
                           \\ gvs [eval_to_Value, LIST_REL_EL_EQN, Abbr ‘argL1’, Abbr ‘argL2’]
                           \\ rpt $ last_x_assum $ qspec_then ‘LENGTH eL2’ assume_tac
                           \\ gvs [EL_MAP2, EL_APPEND_EQN, EL_MAP, eval_to_Value]))
-                \\ qspecl_then [‘argL1'’, ‘valL2’, ‘y2’, ‘k  - 2’] mp_tac eval_to_Apps_Div_or_INR \\ gvs []
+                \\ qmatch_goalsub_abbrev_tac ‘_ (INL Diverge) (eval_to _ (Apps expr2 _))’
+                \\ qspecl_then [‘argL1'’, ‘valL2’, ‘expr2’, ‘k  - 2’] mp_tac eval_to_Apps_Div_or_INR \\ gvs []
                 \\ impl_tac >- gvs [Abbr ‘argL1'’, LIST_REL_EL_EQN, Abbr ‘argL2’]
                 \\ rw [] \\ gvs []
-                \\ rename1 ‘Apps y2 (MAP Value vL2)’
-                \\ Cases_on ‘eval_to (k - 2) (Apps y2 (MAP Value vL2)) = INL Diverge’ \\ gs []
+                \\ rename1 ‘_ (INL Diverge) (eval_to _ (Apps _ (MAP Value valL2')))’
+                \\ Cases_on ‘eval_to (k - 2) (Apps expr2 (MAP Value valL2')) = INL Diverge’ \\ gs []
                 \\ dxrule_then assume_tac eval_to_mono
-                \\ last_x_assum $ qspecl_then [‘k - 2’, ‘Apps x2 (MAP Value valL2)’, ‘Apps y2 (MAP Value vL2)’]
-                                mp_tac
+                \\ last_x_assum $ qspecl_then [‘k - 2’, ‘Apps expr1 (MAP Value valL2)’,
+                                               ‘Apps expr2 (MAP Value valL2')’] mp_tac
                 \\ gvs [] \\ impl_tac \\ gvs []
-                \\ irule exp_rel_Apps \\ gvs [LIST_REL_EL_EQN, EL_MAP]
-                \\ rw [exp_rel_def] \\ gvs [])
+                \\ irule exp_rel_Apps \\ gvs [LIST_REL_EL_EQN, EL_MAP, exp_rel_def]
+                \\ gvs [Abbr ‘expr1’, Abbr ‘expr2’]
+                \\ irule exp_rel_Apps
+                \\ conj_tac
+                >- (irule exp_rel_Apps \\ gvs [EVERY2_MAP, subst1_def, exp_rel_def]
+                    \\ qspecl_then [‘λx y. v_rel (SND x) (SND y)’, ‘λx.x’]
+                                   assume_tac $ GEN_ALL LIST_REL_FILTER
+                    \\ gs [GSYM FST_THM] \\ pop_assum irule \\ gvs [MAP_ZIP]
+                    \\ irule LIST_REL_mono
+                    \\ qexists_tac ‘λx y. v_rel (SND x) (SND y)’ \\ gvs []
+                    \\ gvs [LIST_REL_EL_EQN, EL_ZIP])
+                \\ IF_CASES_TAC \\ gvs [subst1_def, exp_rel_def])
+
             \\ Q.REFINE_EXISTS_TAC ‘j + j1 + j2’ \\ gvs []
             \\ ‘eval_to (j + k) y ≠ INL Diverge’ by gvs []
             \\ dxrule_then assume_tac eval_to_mono \\ gvs []
